Specialize DB to positive to work around strict positivity. Fix various bugs

src/Utils/RelationalDB.v
@@ -7,12 +7,15 @@
 Require Import Equalities Orders ZArith List.
 Import ListNotations.
 From coqutil Require Import Map.Interface.
-From Utils Require Import Utils Natlike ArrayList ExtraMaps.
+From coqutil Require Map.SortedList.
+Require Import Tries.Canonical.
+From Utils Require Import Utils Natlike ArrayList ExtraMaps NatlikePos.
+From Utils Require TrieMap.
 Import Sets.
 
-Section QueryTrie.
 
-  Context (A : Type).
+Open Scope positive.
+
   
   (*TODO: determine whether to generalize idx/elt or just use positive*)
   (* PTree has positive keys, which means elt = positive to use it
@@ -22,155 +25,22 @@ Section QueryTrie.
     depending on how it's generated
    *)
   Inductive query_trie :=
-  | qt_nil
-  (* TODO: use map from A to tries?
-     Currently includes duplication
-     TODO: need to expose map impl or inductive is not strictly positive
-   *)
-  | qt_tree : @named_list A query_trie -> query_trie.
+  (*TODO!!!: what is the difference between qt_nil and qt_tree []
+  | qt_nil*)
+  (* need to expose map impl or inductive is not strictly positive *)
+  | qt_tree : TrieMap.map query_trie -> query_trie.
 
+  Notation qt_nil := (qt_tree (PTree.Empty)).
   
-  Definition values_of_next_var (t : query_trie) : list A :=
-    match t with
-    | qt_tree l => map fst l
-    | _ => []
-    end.
-
-  Context `{Eqb A}.
+  Definition values_of_next_var (t : query_trie) :  list positive :=
+    let (m) := t in
+    map.fold (fun l k _ => cons k l) [] m.
   
-  Definition choose_next_val (v:A) (t : query_trie) : query_trie :=
-    match t with
-    | qt_nil => qt_nil
-    | qt_tree l => named_list_lookup qt_nil l v
-    end.
+  Definition choose_next_val (v:positive) (t : query_trie) : query_trie :=
+    let (m) := t in
+    match map.get m v with Some t => t | None => qt_nil end.
+    
 
-End QueryTrie.
-
-Arguments values_of_next_var {_}.
-Arguments choose_next_val {_}%type {_}.
-
-Arguments qt_nil {_}%type_scope.
-Arguments qt_tree {_}%type_scope _.
-
-
-Section WithIdx.
-  (*Idx type used for relation ids and variables *)
-  Context (Idx : Type) {natlike_idx : Natlike Idx}.
-  (* elt is the type of elements of a relation *)
-  Context (elt : Type) {elt_eqb : Eqb elt}
-          {elt_default : WithDefault elt (*not necessary, just convenient*)}.
-
-  (*invariant: all lists have the same length
-   *)
-  Context {relation : set (list elt)}.
-
-  (* We distinguish the relation id as a key for efficiency *)
-  Context {db : map.map Idx relation}.
-
-  (* We establish a type for conjunctive queries *)
-
-  (*TODO: use primitive pair?*)
-  Definition atom : Type := Idx (*Relation id*) * list Idx.
-  Record query :=
-    {
-      free_vars : list Idx;
-      (*TODO: list or set?*)
-      clauses : list atom;
-    }.
-
-
-
-  Context {arg_map : map.map Idx elt}
-          {id_set : set Idx}
-          {elt_set : set elt}.
-  (* TODO: figure out whether this can have duplicates
-     {subst_set : set arg_map}.
-   *)
-  Definition subst_set := list arg_map.
-
-
-  Fixpoint generic_join' (tries : @named_list Idx (query_trie elt))
-           (vars : list Idx) (acc : arg_map) : subst_set :=
-    match vars with
-    | [] => [acc]
-    | (x::vars') =>
-        let Dx := fold_left (fun l '(_,v) => (values_of_next_var v)++l) tries [] in
-        flat_map (fun v => generic_join' (named_map (choose_next_val v) tries) vars'
-                                         (map.put acc x v))
-                 Dx
-    end.
-  
-
-  (* we need constants for residual queries in generic_join *)
-  Variant argument := const_arg (c : elt) | var_arg (x : Idx).
-
-  Fixpoint match_args_put (x : Idx) (e : elt) l :=
-    match l with
-    | [] => [(x,e)]
-    | (x',e') ::l =>
-        if eqb x x' then if eqb e e' then (x',e')::l else []
-        else (x',e')::(match_args_put x e l)
-    end.
-  
-  Fixpoint match_args args tuple :=
-    match args, tuple with
-    | [], _ => []
-    | _,[] => []
-    | (var_arg x)::args, e::tuple =>
-        match_args_put x e (match_args args tuple)
-    | (const_arg c)::args, e::tuple =>
-        if eqb c e then match_args args tuple else []
-    end.
-
-
-  Definition find_values_in_relation x (rel : relation) args :=
-    map.fold (fun acc tuple _ =>
-                match named_list_lookup_err (match_args args tuple) x with
-                | Some e => e::acc
-                | _ => acc
-                end) [] rel.
-
-  Definition arg_subst v x a :=
-    match a with
-    | const_arg c => const_arg c
-    | var_arg x' =>
-        if eqb x x' then const_arg v else var_arg x'
-    end.
-  
-  (*TODO: filter rel on recursive calls?*)
-  Fixpoint build_trie' (rel: relation) (vars : list Idx) (args : list argument) : (query_trie elt) :=
-    match vars with
-    | [] => qt_nil
-    | x::vars' =>
-        let vs := find_values_in_relation x rel args in
-        qt_tree (map (fun v => (v, build_trie' rel vars' (map (arg_subst v x) args))) vs)
-    end.
-
-  Definition build_trie (d:db) (vars : list Idx) (clause : atom) : Idx * (query_trie elt) :=
-    let rel_id := fst clause in
-    match map.get d rel_id with
-    | Some rel => (rel_id,build_trie' rel vars (map var_arg (snd clause)))
-    | None => (rel_id, qt_nil)
-    end.
-  
-  Definition build_tries (d:db) (vars : list Idx) (clauses : list atom) : @named_list Idx (query_trie elt) :=
-    map (build_trie d vars) clauses.
-           
-  Definition generic_join (d : db) (q : query) : subst_set :=
-    let tries := build_tries d q.(free_vars) q.(clauses) in
-    generic_join' tries q.(free_vars) map.empty.
-  
-End WithIdx. 
-
-Arguments generic_join {_}%type {_} {_}%type {_ _ _ _} _ _.
-Arguments free_vars {_}%type.
-Arguments clauses {_}%type.
-
-
-From coqutil Require Map.SortedList.
-From Utils Require TrieMap NatlikePos.
-
-Module MinimalPositiveInstantiation.
 
   Fixpoint list_compare l1 l2 :=
     match l1, l2 with
@@ -208,13 +78,120 @@ Module MinimalPositiveInstantiation.
 
   Definition db : map.map positive relation := TrieMap.map _.
 
-  Notation query := (query positive).
-
   Definition arg_map : map.map positive positive := TrieMap.map _.
-  
-  Definition generic_join : db -> query -> list arg_map :=
-    @generic_join _ _ _ _ _ _ _.
 
+  Definition Idx := positive.
+  Definition elt := positive.
+
+  (* We establish a type for conjunctive queries *)
+
+  (*TODO: use primitive pair?*)
+  Definition atom : Type := Idx (*Relation id*) * list Idx.
+  Record query :=
+    {
+      free_vars : list Idx;
+      (*TODO: list or set?*)
+      clauses : list atom;
+    }.
+
+
+
+  (* TODO: figure out whether this can have duplicates
+     {subst_set : set arg_map}.
+   *)
+  Definition subst_set := list arg_map.
+
+  Fixpoint generic_join' (tries : @named_list Idx query_trie)
+           (vars : list Idx) (acc : arg_map) : subst_set :=
+    match vars with
+    | [] => [acc]
+    | (x::vars') =>
+        let Dx := flat_map (fun '(_,v) => values_of_next_var v) tries in
+        flat_map (fun v => generic_join' (named_map (choose_next_val v) tries) vars'
+                                         (map.put acc x v))
+                 Dx
+    end.
+  
+
+  (* we need constants for residual queries in generic_join *)
+  Variant argument := const_arg (c : elt) | var_arg (x : Idx).
+
+Require Import Utils.Monad.
+Fixpoint match_args args tuple : option arg_map :=
+  match args, tuple with
+  | [], _ => Some map.empty
+  | _,[] => Some map.empty
+  | (var_arg x)::args, e::tuple =>
+      @! let m <- match_args args tuple in
+         match map.get m x with
+         | Some e' => if eqb e e' then Some m else None
+         | None => Some (map.put m x e)
+         end
+  | (const_arg c)::args, e::tuple =>
+      if eqb c e then match_args args tuple else None
+  end.
+
+Goal match_args [var_arg 1;var_arg 1;var_arg 1] [2; 3; 4] = None.
+  reflexivity.
+Qed.
+
+Goal (Mbind (fun m => map.get m 1) (match_args [var_arg 1;var_arg 1;var_arg 1] [3; 3; 3]) = Some 3).
+  reflexivity.
+Qed.
+
+
+Definition match_args_and_lookup args tuple (x : Idx) : option elt :=
+  @! let m <- match_args args tuple in
+     let e <- map.get m x in
+     ret e.
+
+  Definition find_values_in_relation (x : Idx) (rel : relation) args :=
+    map.fold (fun acc tuple _ =>
+                match match_args_and_lookup args tuple x with
+                | Some e => e::acc
+                | None => acc
+                end) [] rel.
+
+  Definition arg_subst v x a :=
+    match a with
+    | const_arg c => const_arg c
+    | var_arg x' =>
+        if eqb x x' then const_arg v else var_arg x'
+    end.
+
+Goal (arg_subst 2 1 (var_arg 1) = const_arg 2). reflexivity. Qed.
+Goal (arg_subst 2 1 (var_arg 3) = var_arg 3). reflexivity. Qed.
+Goal (arg_subst 2 1 (const_arg 1) = const_arg 1). reflexivity. Qed.
+  
+  (*TODO: filter rel on recursive calls?*)
+Fixpoint build_trie' (rel: relation) (vars : list Idx) (args : list argument)
+  : query_trie :=
+    match vars with
+    | [] => qt_nil
+    | x::vars' =>
+        let vs := find_values_in_relation x rel args in
+        qt_tree (fold_left
+                   (fun m v =>
+                      map.put m v (build_trie' rel vars' (map (arg_subst v x) args)))
+                   vs
+                   map.empty)
+    end.
+
+  Definition build_trie (d:db) (vars : list Idx) (clause : atom) : Idx * query_trie :=
+    let rel_id := fst clause in
+    match map.get d rel_id with
+    | Some rel => (rel_id,build_trie' rel vars (map var_arg (snd clause)))
+    | None => (rel_id, qt_nil)
+    end.
+  
+Definition build_tries (d:db) (vars : list Idx) (clauses : list atom)
+  : @named_list Idx query_trie :=
+    map (build_trie d vars) clauses.
+           
+  Definition generic_join (d : db) (q : query) : subst_set :=
+    let tries := build_tries d q.(free_vars) q.(clauses) in
+    generic_join' tries q.(free_vars) map.empty.
+  
   Module Examples.
     Open Scope positive.
 
@@ -225,6 +202,17 @@ Module MinimalPositiveInstantiation.
            [10; 20; 20])
         [6; 4; 5].
 
+
+    Goal find_values_in_relation 1 r1 [var_arg 1; var_arg 2; var_arg 1] = [].
+      Proof. reflexivity. Qed.
+    Goal find_values_in_relation 1 r1 [var_arg 1; var_arg 2; var_arg 3] = [6; 10].
+      Proof. reflexivity. Qed.
+    Goal find_values_in_relation 1 r1 [var_arg 2; var_arg 1; var_arg 1] = [20].
+      Proof. reflexivity. Qed.
+    Goal find_values_in_relation 1 r1 [var_arg 1; var_arg 1; var_arg 2] = [].
+      Proof. reflexivity. Qed.
+    Goal find_values_in_relation 1 r1 [var_arg 1; var_arg 1; var_arg 1] = [].
+      Proof. reflexivity. Qed.
     
     Definition r2 : relation :=
       Sets.add_elt
@@ -241,7 +229,7 @@ Module MinimalPositiveInstantiation.
         (Sets.add_elt
            map.empty
            [10; 20; 30])
-        [4; 4; 8].
+        [4; 4; 5].
     
     Definition db_ex : db :=
       Eval compute in (map.put
@@ -253,21 +241,20 @@ Module MinimalPositiveInstantiation.
                          3 r3).
 
     Definition q1 : query :=
-      Build_query _
-                  [(*1; 2; 3;*) 1; 2]
-                  [(*(1,[1;2;3]); *)(2, [1;2])].
-
-
-    Compute (build_tries _ _ db_ex q1.(free_vars) q1.(clauses)). 
+      Build_query [1;2;3]
+                  [(1,[1;2;3]);(3,[2;2;3])].
+ 
     
     Definition as_list {A} :=
       TrieMap.trie_fold (B:=A) (fun m k v => (k,v)::m) [].
-    (*TODO: duplicates some results; should actually use a set?*)
-    (*TODO: seems bugged on 2nd clause*)
-    Compute (map as_list (generic_join db_ex q1)).
 
-  End Examples.
-           
-  
-End MinimalPositiveInstantiation.
+    Definition tries := Eval compute in  (build_tries db_ex q1.(free_vars) q1.(clauses)).
+
+    Compute (map as_list (generic_join' tries q1.(free_vars) map.empty)).
+    
+    (*TODO: duplicates some results; should actually use a set?
+      Variable ordering seems to affect this
+     *)
+    (*TODO: bug when a var isn't mentioned in all clauses*)
+    Compute (map as_list (generic_join db_ex q1)).
 
